MoreList.thy
@@ -31,6 +31,32 @@ proof-
     by auto
 qed
 
+lemma filter'':
+  assumes "distinct xs" "x \<in> set xs" "P x"  "\<forall> x' \<in> set xs. (P x' \<and> x' \<noteq> x) \<longleftrightarrow> P' x'"
+  shows "\<exists> Pxs1 Pxs2. filter P' xs = Pxs1 @ Pxs2 \<and> filter P xs = Pxs1 @ [x] @ Pxs2"
+proof-
+  obtain xs1 xs2 where "xs = xs1 @ [x] @ xs2" using \<open>x \<in> set xs\<close>
+    by (metis append_eq_Cons_conv self_append_conv2 split_list)
+  let ?Pxs1 = "filter P xs1" and ?Pxs2 = "filter P xs2"
+  have "filter P' xs = ?Pxs1 @ ?Pxs2"
+  proof (rule filter')
+    show "filter P xs = ?Pxs1 @ [x] @ ?Pxs2"
+      using \<open>xs = xs1 @ [x] @ xs2\<close> \<open>P x\<close>
+      by auto
+  next
+    show "x \<notin> set (?Pxs1 @ ?Pxs2)"
+    using \<open>xs = xs1 @ [x] @ xs2\<close> \<open>distinct xs\<close>
+    by auto
+  next
+    show "\<forall> x' \<in> set xs. (P x' \<and> x' \<noteq> x) \<longleftrightarrow> P' x'"
+      by fact
+  qed
+  then show ?thesis
+    using \<open>xs = xs1 @ [x] @ xs2\<close> \<open>P x\<close>
+    by auto
+qed
+
+
 lemma append_subset: 
   assumes "xs @ ys = xs' @ ys'"
   assumes "length ys' \<ge> length ys"
@@ -62,5 +88,44 @@ lemma sum_list_filter_P_notP:
   shows "sum_list (map f xs) = 
          sum_list (map f (filter (\<lambda> x. P x) xs)) + sum_list (map f (filter (\<lambda> x. \<not> P x) xs))"
   by (induction xs) auto
+
+lemma twiceInFilter:
+  assumes "filter P xs = y1 @ [x] @ y2 @ [x] @ y3"
+  shows "\<exists> z1 z2 z3. xs = z1 @ [x] @ z2 @ [x] @ z3"
+  using assms
+proof-
+  let ?P = "filter P xs"
+  have "x \<in> set xs \<and> P x"
+    using assms
+    by (metis append_Cons filter_set in_set_conv_decomp member_filter)
+  then obtain xs1 xs2 where "xs = xs1 @ [x] @ xs2"
+    by (metis append_eq_Cons_conv eq_Nil_appendI remove1_split)
+  have "x \<in> set xs1 \<union> set xs2"
+  proof (rule ccontr)
+    assume "\<not> ?thesis"
+    then have "?P = (filter P xs1) @ [x] @ (filter P xs2)" "x \<notin> set (filter P xs1)" "x \<notin> set (filter P xs2)"
+      using \<open>xs = xs1 @ [x] @ xs2\<close>  \<open>x \<in> set xs \<and> P x\<close>
+      by auto
+    then show False
+      using assms
+      by (metis append_Cons append_Cons_eq_iff append_Nil in_set_conv_decomp)
+  qed
+  then show ?thesis
+  proof
+    assume "x \<in> set xs1"
+    then obtain xs1' xs1'' where "xs1 = xs1' @ [x] @ xs1''"
+      by (metis append_Cons append_Nil in_set_conv_decomp)
+    then show ?thesis
+      using \<open>xs = xs1 @ [x] @ xs2\<close>
+      by auto
+  next
+    assume "x \<in> set xs2"
+    then obtain xs2' xs2'' where "xs2 = xs2' @ [x] @ xs2''"
+      by (metis append_Cons append_Nil in_set_conv_decomp)
+    then show ?thesis
+      using \<open>xs = xs1 @ [x] @ xs2\<close>
+      by auto
+  qed
+qed
 
 end
